

Proposition 1 (The inclusion exclusion principle.). *For finite sets A_1, A_2, \dots, A_M finite sets,*

$$\left| \bigcup_{j=1}^M A_j \right| = \sum_{\emptyset \neq I \subseteq \{1, 2, \dots, M\}} (-1)^{|I|-1} \left| \bigcap_{j \in I} A_j \right|.$$

Proof. The case of one set is trivial, and the case of two sets is the familiar and easily justified statement that $|A_1 \cup A_2| = |A_1| + |A_2| - |A_1 \cap A_2|$. Proceeding inductively, for $M \geq 3$, assume the result for $M-1$ sets, where and let us prove it for M sets. Let us split up the sum on the right into those sets I that do not contain M and those that do. By our inductive hypothesis, the first sum equals $\left| \bigcup_{j=1}^{M-1} A_j \right|$ and the second sum can be written as $\sum_{\{M\} \subseteq I \subseteq \{1, 2, \dots, M\}} (-1)^{|I|-1} \left| \bigcap_{j \in I} A_j \right|$. Separating out the term with $I = \{M\}$, this equals $|A_M| - \sum_{\emptyset \neq I \subseteq \{1, 2, \dots, M-1\}} (-1)^{|I|} \left| \bigcap_{j \in I} (A_j \cap A_M) \right|$. Again using our inductive hypothesis, the sum here $\left| \bigcup_{j=1}^{M-1} (A_j \cap A_M) \right| = \left| \left(\bigcup_{j=1}^{M-1} A_j \right) \cap A_M \right|$. The entire right side of our desired equation therefore equals $\left| \bigcup_{j=1}^{M-1} A_j \right| + |A_M| - \left| \left(\bigcup_{j=1}^{M-1} A_j \right) \cap A_M \right|$. By the case of our proposition with two sets, this equals $\left| \bigcup_{j=1}^M A_j \right|$, as desired. \square

Proof. The case of one set is trivial, and the case of two sets is the familiar and easily justified statement that $|A_1 \cup A_2| = |A_1| + |A_2| - |A_1 \cap A_2|$. Proceeding by induction, for $M \geq 2$, we prove the case of $M+1$ sets using the case of 2 sets and the case of M sets.

$$\begin{aligned} \left| \bigcup_{j=1}^{M+1} A_j \right| &= \left| \bigcup_{j=1}^M A_j \right| + |A_{M+1}| - \left| \left(\bigcup_{j=1}^M A_j \right) \cap A_{M+1} \right| \\ &= \left| \bigcup_{j=1}^M A_j \right| + |A_{M+1}| - \left| \bigcup_{j=1}^M (A_j \cap A_{M+1}) \right| \\ &= \left| \bigcup_{j=1}^M A_j \right| + |A_{M+1}| - \sum_{\emptyset \neq I \subseteq \{1, 2, \dots, M\}} (-1)^{|I|-1} \left| \bigcap_{j \in I} (A_j \cap A_{M+1}) \right| \\ &= \left| \bigcup_{j=1}^M A_j \right| + |A_{M+1}| - \sum_{\emptyset \neq I \subseteq \{1, 2, \dots, M\}} (-1)^{|I|-1} \left| \left(\bigcap_{j \in I} A_j \right) \cap A_{M+1} \right| \\ &= \left| \bigcup_{j=1}^M A_j \right| + \sum_{\{M+1\} \subseteq I \subseteq \{1, 2, \dots, M+1\}} (-1)^{|I|-1} \left| \bigcap_{j \in I} (A_j \cap A_{M+1}) \right| \end{aligned}$$

Proceeding by induction, for $M \geq 2$, we prove the case of $M+1$ sets by first using the case of 2 sets to get

$$(*) \quad \left| \bigcup_{j=1}^{M+1} A_j \right| = \left| \bigcup_{j=1}^M A_j \right| + |A_{M+1}| - \left| \left(\bigcup_{j=1}^M A_j \right) \cap A_{M+1} \right|.$$

Noticing that $\left(\bigcup_{j=1}^M A_j\right) \cap A_{M+1} = \bigcup_{j=1}^M (A_j \cap A_{M+1})$, the case of M sets gives us

$$-\left|\left(\bigcup_{j=1}^M A_j\right) \cap A_{M+1}\right| = \sum_{\emptyset \neq I \subseteq \{1,2,\dots,M\}} (-1)^{|I|} \left|\bigcap_{j \in I} (A_j \cap A_{M+1})\right|.$$

This right side of this equals $\sum_{\emptyset \neq I \subseteq \{1,2,\dots,M\}} (-1)^{|I|} \left|\left(\bigcap_{j \in I} A_j\right) \cap A_{M+1}\right|$ and therefore equals $\sum_{\{M+1\} \neq I \subseteq \{1,2,\dots,M+1\}} (-1)^{|I|-1} \left|\bigcap_{j \in I} A_j\right|$. Now again using our inductive hypothesis to get $\left|\bigcup_{j=1}^M A_j\right| = \sum_{\emptyset \neq I \subseteq \{1,2,\dots,M\}} (-1)^{|I|-1} \left|\bigcap_{j \in I} A_j\right|$, the right side of (*) equals $\sum_{\emptyset \neq I \subseteq \{1,2,\dots,M\}} (-1)^{|I|-1} \left|\bigcap_{j \in I} A_j\right|$, as desired. \square

Proposition 2 (The inclusion exclusion principle.). *Consider finitely many subsets A_j , where $j \in J$, of a finite set S . Then*

$$\left|S \setminus \left(\bigcup_{j \in J} A_j\right)\right| = \sum_{I \subseteq J} (-1)^{|I|} \left|\bigcap_{j \in I} A_j\right|,$$

where we consider $\bigcap_{j \in I} A_j$ to be equal to S when I is the empty set.

Proof. Fix $s \in S$. We consider which sets s is in, and how this contributes to the expressions on the left and right side of our desired equation.

If $s \notin \bigcup_{j \in J} A_j$, i.e., $s \in S \setminus \left(\bigcup_{j \in J} A_j\right)$, then s contributes 1 to the left side. Since $s \notin \bigcap_{j \in I} A_j$ for all nonempty $I \subseteq J$, we have that s contributes to the right side only when I is the empty set, and since the size of the empty set is zero and $(-1)^0 = 1$, s contributes 1 to the right side.

Now suppose $s \in \bigcup_{j \in J} A_j$, so that s contributes 0 to the left side. Let $A_{j_1}, A_{j_2}, \dots, A_{j_n}$ be the distinct sets A_j that contain s . We then have $n \geq 1$. To see that s contributes 0 to the sum on the right side, first notice that $s \in \bigcap_{j \in I} A_j$ if and only if $I \subseteq \{j_1, j_2, \dots, j_n\}$. For each subset $I \subseteq \{j_1, j_2, \dots, j_n\}$, the contribution due to s is positive when $|I|$ is even, and negative when $|I|$ is odd. For all nonnegative integers $k \leq n$, there are $\binom{n}{k}$ subsets of $\{j_1, j_2, \dots, j_n\}$ of size k , so the contribution of s to the right side is $\sum_{k=0}^n (-1)^k \binom{n}{k} = (1-1)^n = 0$. \square

The other way...

Proposition 3 (The inclusion exclusion principle.). *Let J be a finite set, and for each $j \in J$, let A_j be a finite set. Then*

$$\left|\bigcup_{j \in J} A_j\right| = \sum_{I \subseteq J, I \neq \emptyset} (-1)^{|I|-1} \left|\bigcap_{j \in I} A_j\right|.$$

Proof. Every set appearing in this equation is contained in $\bigcup_{j \in J} A_j$, so let $s \in \bigcup_{j \in J} A_j$. Clearly s contributes 1 to the left side of the equation. To see that it also contributes 1 to the right side, let $\{j_1, j_2, \dots, j_n\}$ be the set of all $j \in J$ such that $s \in A_j$. We have $n \geq 1$ since $s \in \bigcup_{j \in J} A_j$. Also, for any nonempty I with $I \subseteq J$, $s \in \bigcap_{j \in I} A_j$ if and only if $I \subseteq \{j_1, j_2, \dots, j_n\}$. For each nonempty $I \subseteq \{j_1, j_2, \dots, j_n\}$, the contribution on the right side of the equation due to s is negative when $|I|$ is even, and positive when $|I|$ is odd. For all positive integers

$k \leq n$, there are $\binom{n}{k}$ subsets of $\{j_1, j_2, \dots, j_n\}$ of size k , so the contribution of s to the right side is $\sum_{k=1}^n (-1)^{k-1} \binom{n}{k} = 1 - \sum_{k=0}^n (-1)^k \binom{n}{k}$. The binomial theorem tells us $\sum_{k=0}^n (-1)^k \binom{n}{k} = (1-1)^n = 0$, so the contribution of s to the right side is also 1. \square